Work on typing

ERT/Typed/Basic.lean
@@ -1,61 +1,156 @@
 import ERT.Untyped.Basic
 
+open World
+
 structure Var (α) where
-  kind: Kind
   ty: Term α
+  world: World
 
-structure Var.le {α} (a b: Var α): Prop where
-  kind: a.kind.le b.kind
-  ty: a.ty = b.ty
+inductive World.IsMin: World -> World -> World -> Type
+  | ghost_left (w w'): IsMin w ghost w'
+  | ghost_right (w): IsMin ghost comp w
+  | comp: IsMin comp comp comp
 
-inductive Downgrade {α}: List (Var α) -> List (Var α) -> Type
-  | nil: Downgrade [] []
-  | cons: ∀ {x y xs ys}, x.le y -> Downgrade xs ys -> Downgrade (x :: xs) (y :: ys)
+inductive Term.IsSort {α}: Term α -> World -> Type
+  | prop: Term.IsSort prop ghost
+  | type (w): Term.IsSort type w
 
-inductive HasVar {α}: List (Var α) -> ℕ -> Term α -> Type where
-  | head: ∀ {xs x}, x.kind.solid -> HasVar (x :: xs) 0 x.ty
-  | tail: ∀ {xs x y n}, HasVar xs n x -> HasVar (y :: xs) (n + 1) x
+def Term.IsSort.toGhost {α K w}: @Term.IsSort α K w -> Term.IsSort K ghost
+  | prop => prop
+  | type _ => type ghost
 
-inductive Term.HasKind {α}: Term α -> Kind -> Prop where
-  | prop: Term.HasKind Term.prop Kind.prop
-  | type w: Term.HasKind Term.type (Kind.type w)
+inductive HasVar {α}: List (Var α) -> ℕ -> Term α -> World -> Type where
+  | head: ∀ {xs x w}, w.le x.world -> HasVar (x :: xs) 0 x.ty w
+  | tail: ∀ {xs x y n w}, HasVar xs n x w -> HasVar (y :: xs) (n + 1) x w
 
-def Term.IsKind {α}: Term α -> Prop := λt => ∃k, Term.HasKind t k
+def HasVar.toGhost {α Γ n A w}: @HasVar α Γ n A w -> HasVar Γ n A ghost
+  | head _ => head (World.le.ghost _)
+  | tail H => tail H.toGhost
 
-inductive Term.HasType {α}: List (Var α) -> Term α -> Term α -> Type
+inductive Term.PiType {α}: World -> Term α -> Term α -> Term α -> World -> Type
+  | pi (w): PiType comp type type type w
+  | inter (w): PiType ghost type type type w
+  | checked: PiType comp type prop prop ghost
+  | forall_: PiType ghost type prop prop ghost
+  | assume (w): PiType ghost prop type type w
+  | implies: PiType ghost prop prop prop ghost
+
+def Term.PiType.toGhost {α w} {KA KB KC: Term α} {rw}
+  : Term.PiType w KA KB KC rw -> Term.PiType w KA KB KC ghost
+  | pi _ => pi ghost
+  | inter _ => inter ghost
+  | checked => checked
+  | forall_ => forall_
+  | assume _ => assume ghost
+  | implies => implies
+
+-- inductive Term.SigmaType {α}: World -> Term α -> Term α -> Term α -> World -> Type
+--   | sigma (w): SigmaType comp type type type w
+--   | union (w): SigmaType ghost type type type w
+--   | set (w): SigmaType comp type prop type w
+--   | exists_: SigmaType ghost type prop prop ghost
+--   | valid (w): SigmaType ghost prop type type w
+--   | and: SigmaType ghost prop prop prop ghost
+
+-- def Term.SigmaType.toGhost {α w} {KA KB KC: Term α} {rw}
+--   : Term.SigmaType w KA KB KC rw -> Term.SigmaType w KA KB KC ghost
+--   | sigma _ => sigma ghost
+--   | union _ => union ghost
+--   | set _ => set ghost
+--   | exists_ => exists_
+--   | valid _ => valid ghost
+--   | and => and
+
+inductive Term.HasType {α}: List (Var α) -> Term α -> Term α -> World -> Type
   -- Variables
-  | var {Γ n A}: HasVar Γ n A -> HasType Γ (var n) A
+  | var {Γ n A KA w}: HasVar Γ n A w
+    -> HasType Γ A KA w -> IsSort KA w
+    -> HasType Γ (var n) A w
 
-  -- Type/proposition formers
-  | pi {Γ k A KA B KB}:
-    HasType Γ A KA -> HasKind KA k
-    -> HasType (⟨k, A⟩ :: Γ) B KB
-    -> HasType Γ (Term.pi k A B) KB
-  | sigma {Γ k A KA B KB KC}:
-    HasType Γ A KA -> Term.HasKind KA k
-    -> HasType (⟨k, A⟩ :: Γ) B KB
-    -> Term.IsKind KC -> HasType Γ (Term.pi k A B) KC
-  | coprod {Γ A B K}
-    : HasType Γ A K -> HasType Γ B K -> HasType Γ (Term.coprod A B) Term.type
+  -- Term/type formers
+  -- NOTE: no need to shift down kind variables in
+  -- The whole IsSort KB w vs IsSort KB rw hack is to cleanly disallow pi (x: comp A) -> φ;
+  -- propositions should only depend on ghosts!
+  | pi
+    : HasType Γ A KA w
+    -> IsSort KA w
+    -> HasType (Var.mk A w :: Γ) B KB rw
+    -> IsSort KB w -- NOTE: IsSort KB rw is implied here!
+    -> HasType Γ (pi w A B) KB rw
+  -- | sigma {Γ w A KA wA B KB wB KC wC}
+  --   : HasType Γ A KA wA
+  --   -> HasType (Var.mk A w :: Γ) B KB wB
+  --   -> SigmaType w KA KB KC wC
+  --   -> HasType Γ (sigma w A B) KB wC
+  -- | coprod {Γ K A wA B wB wC}
+  --   : HasType Γ A K wA -> HasType Γ B K wB -> HasType Γ (coprod A B) K wC
 
   -- Base types
-  | unit: HasType Γ unit type
-  | nat: HasType Γ nat type
-  | prop: HasType Γ prop type
+  | unit (Γ w): HasType Γ unit type w
+  | nat (Γ w): HasType Γ nat type w
+  | prop (Γ): HasType Γ prop type ghost
 
   -- Base propositions
-  | top: HasType Γ top prop
-  | bot: HasType Γ bot prop
-  | eq {Γ A a b}: HasType Γ A type -> HasType Γ a A -> HasType Γ b A -> HasType Γ (eq a b) prop
+  | top (Γ): HasType Γ top prop ghost
+  | bot (Γ): HasType Γ bot prop ghost
+  | eq: HasType Γ A type wA
+    -> HasType Γ a A wa
+    -> HasType Γ b A wb
+    -> HasType Γ (eq a b) prop ghost
 
   -- Term/proof formers
-  -- | let1 {Γ k A KA B KB a e}
-  --   : HasType Γ A KA -> Term.HasKind KA k
-  --   -> HasType Γ B KB -> Term.IsKind KB
-  --   -> HasType Γ a A -> HasType (⟨k, a⟩ :: Γ) e B
-  --   -> HasType Γ (let1 a e) B
-  | lam {Γ k A KA t B KB}: HasType Γ A KA -> Term.HasKind KA k
-    -> HasType Γ B KB
-    -> HasType (⟨k, a⟩ :: Γ) t B -> HasType Γ (lam k A t) (pi k A B)
-  --TODO: downgrade here?
-  | app {Γ k A B s t}: HasType Γ s (pi k A B) -> HasType Γ t A -> HasType Γ (app s t) B
+  | lam: HasType Γ A KA w -> IsSort KA w
+    -> HasType (Var.mk A w :: Γ) t B rw
+    -> HasType (Var.mk A w :: Γ) B KB w -- NOTE: HasType (Var.mk A w :: Γ) B KB rw is implied here!
+    -> HasType Γ (lam w A t) (pi w A B) rw
+  | app: HasType Γ s (pi pw A B) rw
+    -> HasType Γ t A aw
+    -> B.subst t.subst0 = B'
+    -- -> IsMin pw rw aw
+    -> HasType Γ (app s t) B' rw
+
+def Term.HasType.toGhost {α Γ} {a A: Term α} {w}
+  : Term.HasType Γ a A w -> Term.HasType Γ a A ghost
+  | var Hv HA HK => var Hv.toGhost HA.toGhost HK.toGhost
+  | pi HA HKA HB HKB => pi HA HKA HB.toGhost HKB
+  | unit Γ _ => unit Γ ghost
+  | nat Γ _ => nat Γ ghost
+  | prop Γ => prop Γ
+  | top Γ => top Γ
+  | bot Γ => bot Γ
+  | eq HA Ha Hb => eq HA Ha Hb
+  | lam HA HKA Ht HB => lam HA HKA Ht.toGhost HB
+  | app Hs Ht E => app Hs.toGhost Ht E -- (IsMin.ghost_left _ _)
+
+inductive Term.IsKind {α}: List (Var α) -> Term α -> World -> Type
+  | meta (Γ w): IsKind Γ type w
+  | sort {Γ A K w}: IsSort K w -> HasType Γ A K w -> IsKind Γ A w
+
+abbrev Term.IsKind.type {α Γ A w} (H: @HasType α Γ A type w): IsKind Γ A w :=
+  IsKind.sort (IsSort.type _) H
+
+-- abbrev Term.IsKind.prop {α Γ A w} (H: @HasType α Γ A prop w): IsKind Γ A w :=
+--   IsKind.sort IsSort.prop H
+
+def Term.IsKind.kindSort {α Γ K w w'}: @IsKind α Γ K w -> IsSort K w' -> IsSort K w
+  | _, IsSort.type _ => IsSort.type _
+  | IsKind.sort _ H, IsSort.prop =>
+    have H': w = ghost := by cases H; rfl;
+    H' ▸ IsSort.prop
+
+def Term.IsSort.toKind {α K w} (Γ): @IsSort α K w -> Term.IsKind Γ K w
+  | type _ => IsKind.meta _ _
+  | prop => IsKind.sort (IsSort.type _) (HasType.prop _)
+
+-- def Term.HasType.regular {α Γ} {a A: Term α} {w}
+--   : Term.HasType Γ a A w -> Term.IsKind Γ A w
+--   | var _ HA HK => IsKind.sort HK HA
+--   | pi _ _ HB HKB => (IsKind.kindSort HB.regular HKB).toKind _
+--   | unit _ _ | nat _ _ | prop _ => IsKind.meta _ _
+--   | top _ | bot _ | eq _ _ _ => IsKind.type (HasType.prop _)
+--   | lam HA HKA Ht HB =>
+--     have Hb' := Ht.regular;
+--     match Hb' with
+--     | IsKind.meta _ _ => by cases HB
+--     | IsKind.sort Hb' Hb'' => IsKind.sort sorry (pi sorry sorry sorry)
+--   | app _ _ _ => sorry
